skrrt

Q2.dfy
@@ -1,23 +1,25 @@
 
 method ComputeFact(n : nat) returns (res : nat)
-  requires n > 0;
-  ensures res == fact(n);
+  requires n > 0
+  ensures res == fact(n)
  {
   res := 1;
   var i := 2;
-  while (i <= n) 
+  while (i <= n)
+  invariant res == fact(i - 1)
+  invariant 1 < i <= n + 1
+  // unclear if we need the decreases variant here.
+  decreases n - i
   {
     res := res * i;
     i := i + 1;
   }
  }
 
-method fact(n : nat) returns (res : nat)
-
+// Helper ghost function used to prove ComputeFact
+ghost function fact(n : nat) : nat
+  requires n > 0
+  ensures fact(n) > 0
 {
-  res := n * fact(n-1);
-  if(n == 1){
-    return res;
-  }
-  
+  if(n == 1) then n else fact(n-1) * n
 }
