CircularBuffer.dfy
@@ -1,0 +1,114 @@
+class CircularMemory{
+    
+    var cells : array<int>
+    var read_position : int
+    var write_position : int
+    var isFlipped : bool
+
+
+    constructor Init(cap : int)
+        requires cap > 0
+        ensures Valid()
+        ensures fresh(cells)
+        ensures read_position == 0 && write_position == 0
+        ensures cap == cells.Length
+    {
+        cells := new int[cap];
+        read_position, write_position := 0, 0;
+        isFlipped := false;
+    }
+
+    predicate Valid() 
+        reads this
+    {
+        (read_position >= 0 && read_position < cells.Length) &&
+        (write_position >= 0 && write_position < cells.Length) &&
+        (cells.Length > 0)
+    }
+
+    // A predicate indicating no more Read available
+    predicate isEmpty()
+        reads this
+        requires Valid()
+        ensures Valid()
+    {
+        (read_position == write_position) && !isFlipped
+    }
+
+    //A predicate indicating no more Write should be allowed
+    predicate isFull()
+        reads this
+        requires Valid()
+        ensures Valid()
+    {
+        (read_position == write_position) && isFlipped
+    }
+
+    method Read() returns (isSuccess : bool, content : int)
+        modifies this
+        requires Valid()
+        ensures  Valid()
+        ensures isSuccess  ==> 0 <= old(read_position) < cells.Length
+        ensures isSuccess  ==> content       == cells[old(read_position)]
+        ensures !isSuccess ==> read_position == old(read_position)
+        ensures !isSuccess ==> content       == -100
+    {
+        isSuccess := false;
+        content := -100;
+
+        if(!isEmpty()){
+            // if condition holds the read-pointer will end up on same index as the write-pointer and isFlipped get set to false
+            // which indicates the buffer is empty.
+            if(read_position == cells.Length - 1 && write_position == 0){
+                isFlipped := false;
+            }
+            isSuccess     := true;
+            content       := cells[read_position];
+            read_position := (read_position + 1) % cells.Length;
+            return isSuccess, content;          
+        }else { 
+            return isSuccess, content;
+        }
+    }
+
+    
+    method Write(input : int) returns (isSuccess : bool)
+        modifies this, this.cells
+        requires Valid()
+        ensures  Valid()
+        ensures 0           <= old(write_position) < cells.Length
+        ensures isSuccess   ==> cells[old(write_position)] == input
+        ensures !isSuccess  ==> write_position == old(write_position)
+    {
+        isSuccess := false;
+    
+        if(!isFull()){
+            // if condition holds the write-pointer will end up on same index as the read-pointer and isFlipped get set to true
+            // which indicates the buffer is full.
+            if(write_position == cells.Length - 1 && read_position == 0){
+                isFlipped := true;
+            }
+            isSuccess := true;
+            cells[write_position] := input;
+            write_position := (write_position + 1) % cells.Length;
+            return isSuccess;
+        } else {
+            return isSuccess;
+        } 
+    }
+
+    // Question 3 for Lab 3
+  method DoubleCapacity()
+    modifies ???
+    requires Valid()
+    ensures Valid()
+    ensures cells.Length == 2 * old(cells.Length)
+    ensures read_position == old(read_position)
+    ensures write_position == old(write_position)
+    ensures forall j : int :: 0 <= j < old(cells.Length) ==> cells[j] == old(cells[j])
+    ensures forall j : int :: old(cells.Length) <= j < cells.Length ==> cells[j] == 0
+  {
+    // one or more loops to double the capacity of cells
+    // the most important part is the loop invariants!
+  }
+}
